Reintroduce guards in the syntax (and autosubst) after live discussion this morning

theories/signatures/pi.sig
@@ -3,7 +3,8 @@
 -- Note: in π calculus Channels are Values (so there is just one type)
 
 proc  : Type
-Data : Type
+gproc : Type
+Data  : Type
 
 Value : Type
 Equation : Type
@@ -16,15 +17,16 @@ Inequality : Data -> Data -> Equation
 Or : Equation -> Equation -> Equation
 Not : Equation -> Equation
 
-pr_success : proc
-pr_nil : proc
 pr_rec : (bind proc in proc) -> proc
-pr_choice : proc -> proc -> proc
 pr_par : proc -> proc -> proc
-pr_output : Data  -> Data -> proc -> proc
 pr_res : (bind Data in proc) -> proc
-pr_input : Data -> (bind Data in proc) -> proc
--- pr_res : (bind Data in proc) -> proc
--- pr_input : Data -> (bind Data in proc) -> proc
-pr_tau : proc -> proc
 pr_if_then_else : Equation -> proc -> proc -> proc
+g : gproc -> proc
+
+gpr_success : gproc
+gpr_nil : gproc
+-- note that output was not a guard in CCS
+gpr_output : Data  -> Data -> proc -> gproc
+gpr_input : Data -> (bind Data in proc) -> gproc
+gpr_tau : proc -> gproc
+gpr_choice : gproc -> gproc -> gproc
